src/linear/ListSeq.dfy
@@ -152,11 +152,94 @@ class List<A> {
     }
   }
 
+  static lemma ModelRelationWithSpineAux(spine: seq<Node<A>>, model: seq<A>)
+    requires ModelAux(spine) == model
+    ensures |spine| == |model|
+    ensures forall i | 0 <= i < |spine| :: spine[i].data == model[i]
+  {
+    if spine == [] {
+    } else {
+      ModelRelationWithSpineAux(spine[1..], model[1..]);
+    }
+  }
+
+  lemma ModelRelationWithSpine()
+    requires Valid()
+    ensures |spine| == |Model()|
+    ensures forall i | 0 <= i < |spine| :: spine[i].data == Model()[i]
+  {
+    ModelRelationWithSpineAux(spine, Model());
+  }
+
   function Model(): seq<A>
     reads this, spine
     requires Valid()
   {
     ModelAux(spine)
+  }
+
+  // TODO: remove
+  static function ModelUntilAux(xs: seq<Node<A>>, last: Node<A>): seq<A>
+    reads set x | x in xs :: x`data
+  {
+    if xs == [] || xs[0] == last then
+      []
+    else
+      assert xs[0] in xs;
+      assert forall x | x in xs[1..] :: x in xs;
+      [xs[0].data] + ModelUntilAux(xs[1..], last)
+  }
+
+  // TODO: remove
+  function ModelUntil(last: Node<A>): seq<A>
+    reads this, spine
+  {
+    ModelUntilAux(spine, last)
+  }
+
+  // Private
+  function GetIndex(n: Node<A>): nat
+    reads this, spine
+    requires Valid()
+    requires n in Repr()
+    ensures 0 <= GetIndex(n) < |spine|
+    ensures 0 <= GetIndex(n) < |Model()|
+    ensures spine[GetIndex(n)] == n
+    ensures forall i | 0 <= i < |spine| && spine[i] == n :: i == GetIndex(n)
+  {
+    ModelRelationWithSpine();
+    DistinctSpine();
+    var i :| 0 <= i < |spine| && spine[i] == n;
+    i
+  }
+
+  lemma LastHasLastIndex(last: Node<A>)
+    requires Valid()
+    requires last.next == null
+    requires last in Repr()
+    ensures GetIndex(last) == |spine|-1
+  {
+    var i := GetIndex(last);
+    if i != |spine|-1 {
+      assert spine[i].IsPrevOf(spine[i+1]);
+      assert spine[i].next == spine[i+1];
+      assert spine[i+1] != null;
+      assert spine[i+1] == null;
+      assert false;
+    }
+  }
+
+  lemma PrevHasPrevIndex(prev: Node<A>, node: Node<A>)
+    requires Valid()
+    requires prev in Repr()
+    requires node in Repr()
+    requires prev.IsPrevOf(node)
+    ensures GetIndex(prev) == GetIndex(node)-1
+  {
+    var i := GetIndex(prev);
+    assert prev.next == node;
+    assert spine[i].next == spine[i+1];
+    assert spine[i+1] == node;
   }
 
   constructor()
@@ -329,18 +412,25 @@ class List<A> {
     requires Valid()
     requires mid in Repr()
     ensures Valid()
+    ensures spine == Seq.Insert(mid.next, old(spine), old(GetIndex(mid))+1)
+    ensures Model() == Seq.Insert(x, old(Model()), old(GetIndex(mid))+1)
     ensures mid.next != null
     ensures fresh(mid.next)
     ensures mid.next in spine
     ensures mid.next.next == old(mid.next)
     ensures forall n | n in old(spine) :: n in spine
   {
-    /*GHOST*/ DistinctSpine();
+    { // GHOST
+      DistinctSpine();
+      ModelRelationWithSpine();
+    }
     var n := new Node(x, mid.next);
     mid.next := n;
     { // GHOST
       ghost var i :| 0 <= i < |spine| && spine[i] == mid;
       spine := spine[..i+1] + [n] + spine[i+1..];
+      assert Valid();
+      ModelRelationWithSpine();
     }
   }
 
@@ -351,15 +441,26 @@ class List<A> {
     requires mid in Repr()
     requires mid.next != null
     ensures Valid()
+    ensures spine == Seq.Remove(old(spine), old(GetIndex(mid))+1)
+    // Precondition needed for next line:
+    ensures old(GetIndex(mid))+1 < old(|Model()|)
+    ensures Model() == Seq.Remove(old(Model()), old(GetIndex(mid)+1))
     ensures mid.next == old(mid.next.next)
     ensures forall n | n in old(spine) && n != old(mid.next) :: n in spine
   {
-    /*GHOST*/ DistinctSpine();
+    { // GHOST
+      DistinctSpine();
+      ModelRelationWithSpine();
+    }
     ghost var i :| 0 <= i < |spine| && spine[i] == mid;
     assert spine[i+1] == mid.next;
     assert i+2 < |spine| ==> spine[i+2] == mid.next.next;
     mid.next := mid.next.next;
-    /*GHOST*/ spine := spine[..i+1] + spine[i+2..];
+    { // GHOST
+      spine := spine[..i+1] + spine[i+2..];
+      ModelRelationWithSpine();
+      assert Model() == old(Seq.Remove(Model(), GetIndex(mid)+1));
+    }
   }
 
   // Private method
